Automatically clearbody Delta_specs at start_function of any leaf function (one that does not call other functions)

aes/verif_encryption_LL_loop_body.v
@@ -4,9 +4,30 @@ Require Import aes.aes_encryption_loop_body.
 Require Import aes.bitfiddling.
 Local Open Scope Z.
 
+(*  This almost works, except for the reassoc_seq issue ...
+Definition encryption_loop_body : statement :=
+   ltac:(let body := eval hnf in (fn_body f_mbedtls_aes_encrypt)
+      in match body with
+     context [  Sloop
+                       (Ssequence
+                         (Sifthenelse (Ebinop Ogt (Etempvar _i _) (Econst_int (Int.repr 0) _)  _)
+                             Sskip  Sbreak)
+                       ?S) _ ] => exact S
+    end).
+ *)
+
+Definition encryption_loop_body_Delta DS :=
+ (with_Delta_specs DS
+   (initialized_list
+     [_i; _RK; _X0; _X1; _X2; _X3; _tmp; _b0; _b1; _b2; _b3; _b0__1; _b1__1;
+     _b2__1; _b3__1; _b0__2; _b1__2; _b2__2; _b3__2; _b0__3; _b1__3; _b2__3;
+     _b3__3; _t'4; _t'3; _t'2; _t'1]
+     (func_tycontext f_mbedtls_aes_encrypt Vprog Gprog))).
+
 Definition encryption_loop_body_proof_statement :=
  forall
   (Espec : OracleKind)
+  (DS: PTree.t funspec)
   (ctx input output : val)
   (ctx_sh in_sh out_sh : share)
   (plaintext exp_key : list Z)
@@ -32,12 +53,7 @@ Definition encryption_loop_body_proof_statement :=
   (HeqS12 : S12 = mbed_tls_enc_rounds 12 S0 buf 4)
   (i : Z)
   (H1 : 0 < i <= 6),
-semax
-  (initialized_list
-     [_i; _RK; _X0; _X1; _X2; _X3; _tmp; _b0; _b1; _b2; _b3; _b0__1; _b1__1;
-     _b2__1; _b3__1; _b0__2; _b1__2; _b2__2; _b3__2; _b0__3; _b1__3; _b2__3;
-     _b3__3; _t'4; _t'3; _t'2; _t'1]
-     (func_tycontext f_mbedtls_aes_encrypt Vprog Gprog))
+semax (encryption_loop_body_Delta DS)
   (PROP ( )
    LOCAL (temp _i (Vint (Int.repr i));
    temp _RK
@@ -120,7 +136,8 @@ semax
 Lemma encryption_loop_body_proof: encryption_loop_body_proof_statement.
 Proof.
   unfold encryption_loop_body_proof_statement. intros.
-  unfold encryption_loop_body. abbreviate_semax.
+  unfold encryption_loop_body, encryption_loop_body_Delta.
+  abbreviate_semax.
   pose proof masked_byte_range.
 
   forward. forward. simpl (temp _RK _). rewrite Eq by omega. forward. do 4 forward. forward.
